changes

PiLL/PiLL/Alt.lean
@@ -1,51 +1,32 @@
 import Mathlib.Data.List.Permutation
 import Mathlib.Tactic
-
-abbrev Atom := Nat
-
-inductive Types : Type where
-  | atom (a : Atom)
-  | atomDual (a : Atom)
-  | one
-  | bot
-  | tensor (A B : Types)
-  | parr (A B : Types)
-
-instance : One Types := ⟨Types.one⟩
-instance : Bot Types := ⟨Types.bot⟩
-
-infixr:90 " ⨂ " => Types.tensor
-infixr:90 " ⅋ " => Types.parr
+import PiLL.Framework.model.base
 
 
-def Types.dual : Types → Types
-  | atom a       => atomDual a
-  | atomDual a   => atom a
-  | one          => bot
-  | bot          => one
-  | tensor A B   => parr (dual A) (dual B)
-  | parr A B     => tensor (dual A) (dual B)
 
-postfix:max "ᗮ" => Types.dual
 
-abbrev PName := Nat
+-- De brujin Types and Proc relation needed
 
-inductive Proc : Type where
-  | nil
-  | one (x : PName) (P : Proc)
-  | bot (x : PName) (P : Proc)
-  | par (P Q : Proc)
-  | cut (x y : PName) (P : Proc)
-  | parr (x y : PName) (P : Proc)
-  | tensor (x y : PName) (P : Proc)
 
-notation:80 x "⟦" y "⟧․" P => Proc.tensor x y P
-notation:80 x "⸨" y "⸩․" P => Proc.parr x y P
-notation:80 x "⟦⟧․" P => Proc.one x P
-notation:80 x "⸨⸩․" P => Proc.bot x P
-notation:80 "𝑣⸨"x"," y"⸩"P => Proc.cut x y P
-notation "𝟘" => Proc.nil
-infixr:65 " |ₚ " => Proc.par
+
+
+
+
+
+
+
+
+
+
+
+
+
+
+
+
+
+
+
 
 abbrev Env := List (PName × Types)
 
@@ -55,6 +36,26 @@ infixr:86 " ∶ " => Env.mk
 abbrev Env.merge (Γ Δ : Env) : Env := Γ ++ Δ
 infixl:85 "‚ " => Env.merge
 
+lemma Env.merge_unitL (Γ : Env) : ∅‚ Γ = Γ := by simp
+
+lemma Env.merge_unitR (Γ : Env) : Γ‚ ∅ = Γ := by simp
+
+lemma Env.merge_comm (Γ Δ : Env) : List.Perm (Γ‚ Δ) (Δ‚ Γ) := by
+  exact List.perm_append_comm
+
+lemma Env.merge_assoc (Γ Δ Ξ : Env) : Γ‚ Δ‚ Ξ = Γ‚ (Δ‚ Ξ) := by
+  simp [Env.merge]
+
+lemma Env.merge_rotate_left (Γ : Env) (x : PName × Types) :
+  (x :: Γ).Perm (Γ‚ [x]) := by
+  symm ; apply List.perm_append_singleton
+
+lemma Env.merge_swap (Γ : Env) (x y : PName × Types) :
+  List.Perm (x :: y :: Γ) (y :: x :: Γ) := by
+  symm ; simpa using List.Perm.swap x y Γ
+
+
+
 abbrev HyperEnv := List Env
 
 abbrev HyperEnv.merge (𝒢 ℋ : HyperEnv) : HyperEnv := 𝒢 ++ ℋ
@@ -62,7 +63,29 @@ infixl:55 " |ₕ " => HyperEnv.merge
 
 instance : Coe Env HyperEnv := ⟨fun Γ => ({Γ} : HyperEnv)⟩
 
+lemma HyperEnv.merge_unitL (𝒢 : HyperEnv) : ∅ |ₕ 𝒢 = 𝒢 := by simp
+
+lemma HyperEnv.merge_unitR (𝒢 : HyperEnv) : 𝒢 |ₕ ∅ = 𝒢 := by simp
+
+lemma HyperEnv.merge_comm (𝒢 ℋ : HyperEnv) : List.Perm (𝒢 |ₕ ℋ) (ℋ |ₕ 𝒢) := by
+  exact List.perm_append_comm
+
+lemma HyperEnv.merge_assoc (𝒢 ℋ ℐ : HyperEnv) : 𝒢 |ₕ ℋ |ₕ ℐ = 𝒢 |ₕ (ℋ |ₕ ℐ) := by
+  simp [HyperEnv.merge]
+
+lemma HyperEnv.rotate_left (𝒢 : HyperEnv) (Γ : Env) :
+  (Γ :: 𝒢).Perm (𝒢 ++ Γ) := by
+  symm ; apply List.perm_append_singleton
+
+lemma HyperEnv.merge_swap (𝒢 : HyperEnv) (Γ Δ : Env) :
+  List.Perm (Γ :: Δ :: 𝒢) (Δ :: Γ :: 𝒢) := by
+  symm ; simpa using List.Perm.swap Γ Δ 𝒢
+
+
+
 inductive Typing : Proc → HyperEnv → Prop where
+  ------ Additional Structural and Exchange Rules ------
+
   -- | struct {P Q : Proc} {𝒢 ℋ : HyperEnv} :
   --     Typing P 𝒢 → P ≡ₚ Q → 𝒢.Perm ℋ →
   --     --------------------------------
@@ -77,6 +100,8 @@ inductive Typing : Proc → HyperEnv → Prop where
       Typing P 𝒢 → 𝒢.Perm ℋ →
       ------------------------
       Typing P ℋ
+
+  ----------------- Actual Typing Rules -----------------
 
   | mix₀ :
       Typing 𝟘 ∅
@@ -113,46 +138,6 @@ inductive Typing : Proc → HyperEnv → Prop where
 
 notation:65 "⊢ " P " ∷ " 𝒢 => Typing P 𝒢
 
-
-
-
-lemma Env.merge_unitL (Γ : Env) : ∅‚ Γ = Γ := by simp
-
-lemma Env.merge_unitR (Γ : Env) : Γ‚ ∅ = Γ := by simp
-
-lemma Env.merge_comm (Γ Δ : Env) : List.Perm (Γ‚ Δ) (Δ‚ Γ) := by
-  exact List.perm_append_comm
-
-lemma Env.merge_assoc (Γ Δ Ξ : Env) : Γ‚ Δ‚ Ξ = Γ‚ (Δ‚ Ξ) := by
-  simp [Env.merge]
-
-lemma Env.merge_rotate_left (Γ : Env) (x : PName × Types) :
-  (x :: Γ).Perm (Γ‚ [x]) := by
-  symm ; apply List.perm_append_singleton
-
-lemma Env.merge_swap (Γ : Env) (x y : PName × Types) :
-  List.Perm (x :: y :: Γ) (y :: x :: Γ) := by
-  symm ; simpa using List.Perm.swap x y Γ
-
-lemma HyperEnv.merge_unitL (𝒢 : HyperEnv) : ∅ |ₕ 𝒢 = 𝒢 := by simp
-
-lemma HyperEnv.merge_unitR (𝒢 : HyperEnv) : 𝒢 |ₕ ∅ = 𝒢 := by simp
-
-lemma HyperEnv.merge_comm (𝒢 ℋ : HyperEnv) : List.Perm (𝒢 |ₕ ℋ) (ℋ |ₕ 𝒢) := by
-  exact List.perm_append_comm
-
-lemma HyperEnv.merge_assoc (𝒢 ℋ ℐ : HyperEnv) : 𝒢 |ₕ ℋ |ₕ ℐ = 𝒢 |ₕ (ℋ |ₕ ℐ) := by
-  simp [HyperEnv.merge]
-
-lemma HyperEnv.rotate_left (𝒢 : HyperEnv) (Γ : Env) :
-  (Γ :: 𝒢).Perm (𝒢 ++ Γ) := by
-  symm ; apply List.perm_append_singleton
-
-lemma HyperEnv.merge_swap (𝒢 : HyperEnv) (Γ Δ : Env) :
-  List.Perm (Γ :: Δ :: 𝒢) (Δ :: Γ :: 𝒢) := by
-  symm ; simpa using List.Perm.swap Γ Δ 𝒢
-
-
 lemma Typing.env_comm {P : Proc} {𝒢 : HyperEnv} {Γ Δ : Env} :
   (⊢ P ∷ 𝒢 |ₕ Γ‚ Δ) → (⊢ P ∷ 𝒢 |ₕ Δ‚ Γ) :=
   fun h => Typing.exchange_env h (Env.merge_comm _ _)
@@ -175,6 +160,96 @@ lemma Typing.hyper_comm {P : Proc} {𝒢 ℋ : HyperEnv} :
 
 
 
+inductive TypingStep : {P : Proc} → {𝒢 : HyperEnv} → Typing P 𝒢 → Lbl →
+  {P' : Proc} → {𝒢' : HyperEnv} → Typing P' 𝒢' → Prop where
+  | one
+      {P : Proc} {x : PName} {𝒟 : ⊢ P ∷ ∅} :
+      TypingStep (Typing.one 𝒟) (x⟦⟧) 𝒟
+
+  | tensor
+      {Γ Δ : Env} {P : Proc} {x x': PName} {A B : Types}
+      {𝒟 : ⊢ P ∷ Γ‚ x' ∶ A |ₕ Δ‚ x ∶ B} :
+      TypingStep (Typing.tensor 𝒟) (x⟦x'⟧) 𝒟
+
+  | bot
+      {Γ : Env} {P : Proc} {x : PName} {𝒟 : ⊢ P ∷ Γ} :
+      TypingStep (Typing.bot 𝒟) (x⸨⸩) 𝒟
+
+  | parr
+      {Γ : Env} {P : Proc} {x x' : PName} {A B : Types}
+      {𝒟 : ⊢ P ∷ Γ‚ x' ∶ A‚ x ∶ B} :
+      TypingStep (Typing.parr 𝒟) (x⸨x'⸩) 𝒟
+
+  | par₁
+      {𝒢 ℋ 𝒢': HyperEnv} {P Q P' : Proc} {l : Lbl}
+      {𝒟 : ⊢ P ∷ 𝒢} {𝒟' : ⊢ P' ∷ 𝒢'} {ℰ : ⊢ Q ∷ ℋ}
+      (h : TypingStep 𝒟 l 𝒟') (disj : (l.i) ∩ (Q.f) = ∅) :
+      -----------------------------------------------------
+      TypingStep (Typing.mix 𝒟 ℰ) l (Typing.mix 𝒟' ℰ)
+
+  | par₂
+      {𝒢 ℋ ℋ': HyperEnv} {P Q Q' : Proc} {l : Lbl}
+      {𝒟 : ⊢ P ∷ 𝒢} {ℰ : ⊢ Q ∷ ℋ} {ℰ' : ⊢ Q' ∷ ℋ'}
+      (h : TypingStep ℰ l ℰ') (disj : (l.i) ∩ (P.f) = ∅) :
+      ----------------------------------------------------
+      TypingStep (Typing.mix 𝒟 ℰ) l (Typing.mix 𝒟 ℰ')
+
+  | syn
+      {𝒢 𝒢' ℋ ℋ' : HyperEnv} {P P' Q Q' : Proc} {l l' : Act}
+      {𝒟 : ⊢ P ∷ 𝒢} {𝒟' : ⊢ P' ∷ 𝒢'}
+      {ℰ : ⊢ Q ∷ ℋ} {ℰ' : ⊢ Q' ∷ ℋ'}
+      (h₁ : TypingStep 𝒟 l 𝒟') (h₂ : TypingStep ℰ l' ℰ') :
+      ---------------------------------------------------------
+      TypingStep (Typing.mix 𝒟 ℰ) (l |ₗ l') (Typing.mix 𝒟' ℰ')
+
+  -- | alpha_equiv
+  --     {𝒢 𝒢' : HyperEnv} {P Q Q' : Proc} {l : Lbl}
+  --     {𝒟 : ⊢ P ∷ 𝒢} {ℰ : ⊢ Q ∷ 𝒢} {ℰ' : ⊢ Q' ∷ 𝒢'}
+  --     (h₁ : P =ₐ Q) (h₂ : TypingStep ℰ l ℰ') :
+  --     -----------------------------------------------
+  --     TypingStep 𝒟 l ℰ'
+
+  | one_bot
+      {𝒢: HyperEnv} {Γ : Env} {P P' : Proc} {x y : PName}
+      {𝒟 : ⊢ P ∷  𝒢 |ₕ x ∶ 1 |ₕ Γ‚ y ∶ ⊥} {𝒟' : ⊢ P' ∷ 𝒢 |ₕ Γ}
+      (h : TypingStep 𝒟 (x⟦⟧ |ₗ y⸨⸩) 𝒟') :
+      -------------------------------------------------------
+      TypingStep (Typing.cut (Γ := ∅) 𝒟) (τ) 𝒟'
+
+  | tensor_parr
+      {𝒢 : HyperEnv} {Γ Δ Ξ : Env} {P P' : Proc} {x y x' y' : PName} {A B : Types}
+      {𝒟 : ⊢ P ∷ 𝒢 |ₕ Γ‚ Δ‚ x ∶ A ⨂ B |ₕ Ξ‚ y ∶ Aᗮ ⅋ Bᗮ}
+      {𝒟' : ⊢ P' ∷ 𝒢 |ₕ Γ‚ x ∶ B |ₕ Δ‚ x' ∶ A |ₕ Ξ‚ y ∶ Bᗮ‚ y' ∶ Aᗮ}
+      (h : TypingStep 𝒟 (x⟦x'⟧ |ₗ y⸨y'⸩) 𝒟') :
+      ----------------------------------------------------------------------------
+      TypingStep
+        (Typing.cut 𝒟)
+        (τ)
+        (Typing.cut (by
+          let inner := Typing.cut 𝒟'
+          rw [← Env.merge_assoc] at inner
+          exact inner
+          )
+        )
+
+  | res
+      {𝒢 𝒢': HyperEnv} {Γ Γ' Δ Δ' : Env} {P P' : Proc}
+      {x y : PName} {A : Types} {l : Lbl}
+      {𝒟 : Typing P (𝒢 |ₕ Γ‚ x ∶ A |ₕ Δ‚ y ∶ Aᗮ)}
+      {𝒟' : Typing P' (𝒢' |ₕ Γ'‚ x ∶ A |ₕ Δ'‚ y ∶ Aᗮ)}
+      (h : TypingStep 𝒟 l 𝒟') (disj : l.fresh [x, y]) :
+      --------------------------------------------------
+      TypingStep (Typing.cut 𝒟) l (Typing.cut 𝒟')
+
+
+
+
+
+
+
+
+
+
 -- FIXME: Can't really read what is produced by the Typing.***_comm etc. lemmas
 -- Make it look like the syntax
 example : ⊢ ((10⟦⟧․𝟘) |ₚ (40⸨⸩․30⸨⸩․20⟦⟧․𝟘)) ∷
@@ -192,14 +267,8 @@ example : ⊢ ((10⟦⟧․𝟘) |ₚ (40⸨⸩․30⸨⸩․20⟦⟧․𝟘)) �
 
 
 
-
-
-
-inductive Lbl : Type where
-  | one (x : PName)
-  | bot (x : PName)
-
-inductive ProcStep : Proc → Lbl → Proc → Prop where
-
-
-inductive EnvStep : Env → Lbl → Env → Prop where
+example : ⊢ 10⸨20⸩․10⸨⸩․20⟦⟧․𝟘 ∷ 10 ∶ 1 ⅋ ⊥ := by
+  apply Typing.parr (Γ := ∅)
+  apply Typing.bot
+  apply Typing.one
+  apply Typing.mix₀
